cedar-lean/Cedar/Thm/SymCC/Opt.lean
@@ -1,0 +1,171 @@
+/-
+ Copyright Cedar Contributors
+
+ Licensed under the Apache License, Version 2.0 (the "License");
+ you may not use this file except in compliance with the License.
+ You may obtain a copy of the License at
+
+      https://www.apache.org/licenses/LICENSE-2.0
+
+ Unless required by applicable law or agreed to in writing, software
+ distributed under the License is distributed on an "AS IS" BASIS,
+ WITHOUT WARRANTIES OR CONDITIONS OF ANY KIND, either express or implied.
+ See the License for the specific language governing permissions and
+ limitations under the License.
+-/
+
+import Cedar.SymCC
+import Cedar.SymCCOpt
+import Cedar.Thm.Data.Control
+import Cedar.Thm.Data.Set
+import Cedar.Thm.SymCC.Authorizer
+import Cedar.Thm.SymCC.Opt.CompiledPolicies
+import Cedar.Thm.WellTypedVerification
+
+/-!
+Proofs that the optimized interface in SymCCOpt is equivalent to the unoptimized
+interface in SymCC.
+-/
+
+namespace Cedar.Thm
+
+open Cedar.Spec Cedar.SymCC
+
+/--
+This theorem covers the "happy path" -- showing that if optimized policy
+compilation succeeds, then `enforce` and `enforceCompiledPolicy` are equivalent.
+-/
+theorem enforceCompiledPolicy_eqv_enforce_ok {p wp : Policy} {cp : CompiledPolicy} {Γ : Validation.TypeEnv} :
+  CompiledPolicy.compile p Γ = .ok cp →
+  wellTypedPolicy p Γ = .ok wp →
+  enforce [wp.toExpr] (SymEnv.ofTypeEnv Γ) = enforceCompiledPolicy cp
+:= by
+  simp [enforce, enforceCompiledPolicy]
+  intro h₀ h₁
+  simp [
+    cp_compile_produces_the_right_env h₀,
+    cp_compile_produces_the_right_footprint h₀,
+    cp_compile_produces_the_right_acyclicity h₀,
+    compiled_policy_eq_wtp h₀ h₁,
+  ]
+  simp [footprints]
+  simp [Data.Set.make_make_eqv, List.Equiv, List.subset_def]
+  constructor
+  · intro t h₂
+    cases h₂
+    · left
+      rename_i h₂
+      replace ⟨t', h₂, ht⟩ := h₂ ; subst t ; rename Term => t
+      rw [Data.Set.in_list_iff_in_set] at *
+      rw [Data.Set.mem_mapUnion_iff_mem_exists] at h₂
+      replace ⟨s, hs, h₂⟩ := h₂
+      simp at hs ; subst s
+      simp [Data.Set.mem_map]
+      exists t
+    · right
+      rename_i h₂
+      simp [List.mem_mapUnion_iff_mem_exists] at *
+      replace ⟨s, hs, t', ht', h₂⟩ := h₂ ; subst t ; rename Term => t
+      simp [Data.Set.in_list_iff_in_set, Data.Set.mem_mapUnion_iff_mem_exists] at *
+      exists s
+      simp [hs]
+      exists t
+  · intro t h₂
+    cases h₂
+    · left
+      rename_i h₂
+      simp [Data.Set.in_list_iff_in_set, Data.Set.mem_map] at h₂
+      replace ⟨t', ht', h₂⟩ := h₂ ; subst t ; rename Term => t
+      exists t
+      simp [Data.Set.in_list_iff_in_set, Data.Set.mem_mapUnion_iff_mem_exists]
+      exact ht'
+    · right
+      rename_i h₂
+      rw [List.mem_mapUnion_iff_mem_exists] at *
+      simp only [List.mem_map] at *
+      replace ⟨s, hs, t', ht', h₂⟩ := h₂ ; subst t ; rename Term => t
+      exists s
+      rw [Data.Set.in_list_iff_in_set] at *
+      simp [Data.Set.mem_mapUnion_iff_mem_exists, hs]
+      exists t
+      simp [Data.Set.in_list_iff_in_set, Data.Set.mem_mapUnion_iff_mem_exists, ht']
+
+/--
+This theorem covers the "happy path" -- showing that if optimized policy
+compilation succeeds, then `verifyEvaluate` and `verifyEvaluateOpt` are
+equivalent.
+-/
+theorem verifyEvaluateOpt_eqv_verifyEvaluate_ok {p wp : Policy} {cp : CompiledPolicy} {Γ : Validation.TypeEnv} {φ : Term → Term} :
+  CompiledPolicy.compile p Γ = .ok cp →
+  wellTypedPolicy p Γ = .ok wp →
+  verifyEvaluate φ wp (SymEnv.ofTypeEnv Γ) = .ok (verifyEvaluateOpt φ cp)
+:= by
+  simp [verifyEvaluate, verifyEvaluateOpt]
+  simp [do_eq_ok]
+  intro h₀ h₁
+  simp [enforceCompiledPolicy_eqv_enforce_ok h₀ h₁]
+  exists cp.term ; simp
+  exact (cp_compile_produces_the_right_term h₀ h₁).symm
+
+/--
+This theorem covers the "happy path" -- showing that if optimized policy
+compilation succeeds, then `verifyNeverErrors` and `verifyNeverErrorsOpt` are
+equivalent.
+-/
+theorem verifyNeverErrorsOpt_eqv_verifyNeverErrors_ok {p wp : Policy} {cp : CompiledPolicy} {Γ : Validation.TypeEnv} :
+  CompiledPolicy.compile p Γ = .ok cp →
+  wellTypedPolicy p Γ = .ok wp →
+  verifyNeverErrors wp (SymEnv.ofTypeEnv Γ) = .ok (verifyNeverErrorsOpt cp)
+:= by
+  simp [verifyNeverErrors, verifyNeverErrorsOpt]
+  exact verifyEvaluateOpt_eqv_verifyEvaluate_ok
+
+/--
+If `CompiledPolicy.compile` succeeds, then `wellTypedPolicy` succeeds
+-/
+theorem compile_ok_then_welltypedpolicy_ok {p : Policy} {Γ : Validation.TypeEnv} :
+  Except.isOk (CompiledPolicy.compile p Γ) →
+  Except.isOk (wellTypedPolicy p Γ)
+:= by
+  simp [Except.isOk, Except.toBool]
+  simp [CompiledPolicy.compile, Except.mapError]
+  cases h₀ : wellTypedPolicy p Γ <;> simp
+
+/--
+If `CompiledPolicy.compile` succeeds, then `wellTypedPolicy` succeeds
+-/
+theorem compile_ok_then_exists_wtp {p : Policy} {cp : CompiledPolicy} {Γ : Validation.TypeEnv} :
+  CompiledPolicy.compile p Γ = .ok cp →
+  ∃ wp, wellTypedPolicy p Γ = .ok wp
+:= by
+  intro h₀
+  have h₁ := compile_ok_then_welltypedpolicy_ok (by
+    simp [Except.isOk_iff_exists]
+    exists cp
+  )
+  simp [Except.isOk_iff_exists] at h₁
+  exact h₁
+
+/--
+This theorem covers the "happy path" -- showing that if optimized policy
+compilation succeeds, then `wellTypedPolicy` succeeds and `neverErrors?` and
+`neverErrorsOpt?` are equivalent.
+-/
+theorem neverErrorsOpt?_eqv_neverErrors?_ok {p : Policy} {cp : CompiledPolicy} {Γ : Validation.TypeEnv} :
+  Γ.WellFormed →
+  CompiledPolicy.compile p Γ = .ok cp →
+  ∃ wp,
+    wellTypedPolicy p Γ = .ok wp ∧
+    neverErrorsOpt? cp = neverErrors? wp (SymEnv.ofTypeEnv Γ)
+:= by
+  simp [neverErrors?, neverErrorsOpt?]
+  simp [sat?]
+  intro hwf h₀
+  have ⟨wp, h₁⟩ := compile_ok_then_exists_wtp h₀
+  exists wp ; apply And.intro h₁
+  have ⟨asserts, h₂⟩ := verifyNeverErrors_is_ok hwf h₁
+  simp [h₂]
+  simp [cp_compile_produces_the_right_env h₀]
+  simp [compiled_policy_eq_wtp h₀ h₁]
+  simp [verifyNeverErrorsOpt_eqv_verifyNeverErrors_ok h₀ h₁] at h₂
+  subst asserts ; rfl
