cedar-lean/Cedar/Thm/SymCC/Opt/CompiledPolicies.lean
@@ -1,0 +1,130 @@
+/-
+ Copyright Cedar Contributors
+
+ Licensed under the Apache License, Version 2.0 (the "License");
+ you may not use this file except in compliance with the License.
+ You may obtain a copy of the License at
+
+      https://www.apache.org/licenses/LICENSE-2.0
+
+ Unless required by applicable law or agreed to in writing, software
+ distributed under the License is distributed on an "AS IS" BASIS,
+ WITHOUT WARRANTIES OR CONDITIONS OF ANY KIND, either express or implied.
+ See the License for the specific language governing permissions and
+ limitations under the License.
+-/
+
+import Cedar.SymCC
+import Cedar.SymCCOpt
+import Cedar.Thm.Data.Control
+import Cedar.Thm.Data.Set
+import Cedar.Thm.SymCC.Authorizer
+import Cedar.Thm.WellTypedVerification
+
+/-!
+Some lemmas about `CompiledPolicy` and `CompiledPolicies`.
+-/
+
+namespace Cedar.Thm
+
+open Cedar.Spec Cedar.SymCC
+
+/--
+The `.policy` of a `CompiledPolicy` is exactly the policy produced by `wellTypedPolicy`
+-/
+theorem compiled_policy_eq_wtp {p wp : Policy} {cp : CompiledPolicy} {Γ : Validation.TypeEnv} :
+  CompiledPolicy.compile p Γ = .ok cp →
+  wellTypedPolicy p Γ = .ok wp →
+  cp.policy = wp
+:= by
+  simp [CompiledPolicy.compile, do_eq_ok, Except.mapError]
+  intro p' h₀ t h₁ h₂ ; subst cp ; simp
+  split at h₀ <;> simp_all
+
+/--
+The `.policies` of a `CompiledPolicies` is exactly the policies produced by `wellTypedPolicies`
+-/
+theorem compiled_policies_eq_wtps {ps wps : Policies} {cps : CompiledPolicies} {Γ : Validation.TypeEnv} :
+  CompiledPolicies.compile ps Γ = .ok cps →
+  wellTypedPolicies ps Γ = .ok wps →
+  cps.policies = wps
+:= by
+  simp [CompiledPolicies.compile, do_eq_ok, Except.mapError]
+  intro ps' h₀ t h₁ h₂ ; subst cps ; simp
+  split at h₀ <;> simp_all
+
+theorem cp_compile_produces_the_right_env {p : Policy} {cp : CompiledPolicy} {Γ : Validation.TypeEnv} :
+  CompiledPolicy.compile p Γ = .ok cp →
+  cp.εnv = SymEnv.ofTypeEnv Γ
+:= by
+  simp only [CompiledPolicy.compile, Except.mapError, do_eq_ok, Except.ok.injEq, forall_exists_index, and_imp]
+  intro p' h₀ t h₁ h₂ ; subst h₂
+  simp
+
+theorem cps_compile_produces_the_right_env {ps : Policies} {cps : CompiledPolicies} {Γ : Validation.TypeEnv} :
+  CompiledPolicies.compile ps Γ = .ok cps →
+  cps.εnv = SymEnv.ofTypeEnv Γ
+:= by
+  simp only [CompiledPolicies.compile, Except.mapError, do_eq_ok, Except.ok.injEq, forall_exists_index, and_imp]
+  intro ps' h₀ t h₁ h₂ ; subst h₂
+  simp
+
+theorem cp_compile_produces_the_right_term {p wp : Policy} {cp : CompiledPolicy} {Γ : Validation.TypeEnv} :
+  CompiledPolicy.compile p Γ = .ok cp →
+  wellTypedPolicy p Γ = .ok wp →
+  cp.term = SymCC.compile wp.toExpr (SymEnv.ofTypeEnv Γ)
+:= by
+  simp [CompiledPolicy.compile, do_eq_ok, Except.mapError]
+  intro p' h₀ t h₁ h₂ h₃ ; subst cp ; simp only
+  split at h₀ <;> simp at h₀
+  subst p' ; rename_i wp' h₂
+  simp [h₂] at h₃ ; subst wp'
+  split at h₁ <;> simp_all
+
+theorem cps_compile_produces_the_right_term {ps wps : Policies} {cps : CompiledPolicies} {Γ : Validation.TypeEnv} :
+  CompiledPolicies.compile ps Γ = .ok cps →
+  wellTypedPolicies ps Γ = .ok wps →
+  cps.term = SymCC.isAuthorized wps (SymEnv.ofTypeEnv Γ)
+:= by
+  simp [CompiledPolicies.compile, do_eq_ok, Except.mapError]
+  intro ps' h₀ t h₁ h₂ h₃ ; subst cps ; simp only
+  split at h₀ <;> simp at h₀
+  subst ps' ; rename_i wps' h₂
+  simp [h₂] at h₃ ; subst wps'
+  split at h₁ <;> simp_all
+
+theorem cp_compile_produces_the_right_footprint {p : Policy} {cp : CompiledPolicy} {Γ : Validation.TypeEnv} :
+  CompiledPolicy.compile p Γ = .ok cp →
+  cp.footprint = footprint cp.policy.toExpr cp.εnv
+:= by
+  simp [CompiledPolicy.compile, do_eq_ok]
+  intro p h₀ t h₁ h₂ ; subst cp
+  simp
+
+theorem cps_compile_produces_the_right_footprint {ps : Policies} {cps : CompiledPolicies} {Γ : Validation.TypeEnv} :
+  CompiledPolicies.compile ps Γ = .ok cps →
+  cps.footprint = footprints (cps.policies.map Policy.toExpr) cps.εnv
+:= by
+  simp [CompiledPolicies.compile, do_eq_ok]
+  intro ps h₀ t h₁ h₂ ; subst cps
+  simp
+
+theorem cp_compile_produces_the_right_acyclicity {p : Policy} {cp : CompiledPolicy} {Γ : Validation.TypeEnv} :
+  CompiledPolicy.compile p Γ = .ok cp →
+  cp.acyclicity = cp.footprint.map (SymCC.acyclicity · cp.εnv.entities)
+:= by
+  intro temp ; have hf := cp_compile_produces_the_right_footprint temp ; revert temp
+  simp [CompiledPolicy.compile]
+  simp [do_eq_ok, hf]
+  intro p h₀ t h₁ h₂ ; subst cp
+  simp
+
+theorem cps_compile_produces_the_right_acyclicity {ps : Policies} {cps : CompiledPolicies} {Γ : Validation.TypeEnv} :
+  CompiledPolicies.compile ps Γ = .ok cps →
+  cps.acyclicity = cps.footprint.map (SymCC.acyclicity · cps.εnv.entities)
+:= by
+  intro temp ; have hf := cps_compile_produces_the_right_footprint temp ; revert temp
+  simp [CompiledPolicies.compile]
+  simp [do_eq_ok, hf]
+  intro ps h₀ t h₁ h₂ ; subst cps
+  simp
