cedar-lean/Cedar/Thm/SymCC/Verifier/WellTypedOk.lean
@@ -26,10 +26,10 @@ open Spec SymCC Validation
 /-- `verifyEvaluate` succeeds on sufficiently well-formed inputs. -/
 theorem verifyEvaluate_is_ok {φ : Term → Term} {p p' : Policy} {Γ : TypeEnv}
   (hwf : Γ.WellFormed)
-  (hwt : wellTypedPolicy p Γ = .some p') :
+  (hwt : wellTypedPolicy p Γ = .ok p') :
   ∃ asserts, verifyEvaluate φ p' (SymEnv.ofEnv Γ) = .ok asserts
 := by
-  have ⟨tx, hwt_tx, heq_tx⟩ := wellTypedPolicy_some_implies_well_typed_expr hwt
+  have ⟨tx, hwt_tx, heq_tx⟩ := wellTypedPolicy_ok_implies_well_typed_expr hwt
   simp only [verifyEvaluate]
   have ⟨_, hok, _⟩ := compile_well_typed hwf hwt_tx
   simp only [heq_tx] at hok
@@ -38,10 +38,10 @@ theorem verifyEvaluate_is_ok {φ : Term → Term} {p p' : Policy} {Γ : TypeEnv}
 /-- `compileWithEffect` succeeds on sufficiently well-formed inputs. -/
 theorem compileWithEffect_is_ok (effect : Effect) {p p' : Policy} {Γ : TypeEnv}
   (hwf : Γ.WellFormed)
-  (hwt : wellTypedPolicy p Γ = .some p') :
+  (hwt : wellTypedPolicy p Γ = .ok p') :
   ∃ asserts, compileWithEffect effect p' (SymEnv.ofEnv Γ) = .ok asserts
 := by
-  have ⟨tx, hwt_tx, heq_tx⟩ := wellTypedPolicy_some_implies_well_typed_expr hwt
+  have ⟨tx, hwt_tx, heq_tx⟩ := wellTypedPolicy_ok_implies_well_typed_expr hwt
   simp only [compileWithEffect]
   have ⟨_, hok, _⟩ := compile_well_typed hwf hwt_tx
   simp only [heq_tx] at hok
@@ -51,7 +51,7 @@ theorem compileWithEffect_is_ok (effect : Effect) {p p' : Policy} {Γ : TypeEnv}
 /-- `satisfiedPolicies` succeeds on sufficiently well-formed inputs. -/
 theorem satisfiedPolicies_is_ok (effect : Effect) {ps ps' : Policies} {Γ : TypeEnv}
   (hwf : Γ.WellFormed)
-  (hwt : wellTypedPolicies ps Γ = .some ps') :
+  (hwt : wellTypedPolicies ps Γ = .ok ps') :
   ∃ asserts, satisfiedPolicies effect ps' (SymEnv.ofEnv Γ) = .ok asserts
 := by
   simp only [SymCC.satisfiedPolicies]
@@ -63,25 +63,20 @@ theorem satisfiedPolicies_is_ok (effect : Effect) {ps ps' : Policies} {Γ : Type
     | nil => exists []
     | cons hd tl ih =>
       simp only [List.filterMapM_cons]
-      have hwt_policies := List.mapM_some_implies_all_from_some hwt
+      have hwt_policies := List.mapM_ok_implies_all_from_ok hwt
       have ⟨p, hmem_p, hwt_p⟩ := hwt_policies hd List.mem_cons_self
       have ⟨asserts, hasserts⟩ := compileWithEffect_is_ok effect hwf hwt_p
       simp only [hasserts, bind_pure_comp, Except.bind_ok]
       cases ps with
       | nil => contradiction
       | cons ps_hd ps_tl =>
-        simp only [
-          wellTypedPolicies, List.mapM_cons,
-          Option.pure_def,
-          bind, Option.bind,
-        ] at hwt
+        simp only [wellTypedPolicies, List.mapM_cons, bind, Except.bind, pure, Except.pure] at hwt
         split at hwt
         contradiction
-        simp only at hwt
         split at hwt
         contradiction
         rename_i heq
-        simp only [Option.some.injEq, List.cons.injEq] at hwt
+        simp only [Except.ok.injEq, List.cons.injEq] at hwt
         simp only [hwt.2] at heq
         have ⟨ts_tl, hts_tl⟩ := ih heq
         split
@@ -92,7 +87,7 @@ theorem satisfiedPolicies_is_ok (effect : Effect) {ps ps' : Policies} {Γ : Type
 /-- `isAuthorized` succeeds on sufficiently well-formed inputs. -/
 theorem isAuthorized_is_ok {ps ps' : Policies} {Γ : TypeEnv}
   (hwf : Γ.WellFormed)
-  (hwt : wellTypedPolicies ps Γ = .some ps') :
+  (hwt : wellTypedPolicies ps Γ = .ok ps') :
   ∃ asserts, isAuthorized ps' (SymEnv.ofEnv Γ) = .ok asserts
 := by
   simp only [SymCC.isAuthorized]
@@ -103,8 +98,8 @@ theorem isAuthorized_is_ok {ps ps' : Policies} {Γ : TypeEnv}
 /-- `verifyIsAuthorized` succeeds on sufficiently well-formed inputs. -/
 theorem verifyIsAuthorized_is_ok (φ : Term → Term → Term) {ps₁ ps₁' ps₂ ps₂' : Policies} {Γ : TypeEnv}
   (hwf : Γ.WellFormed)
-  (hwt₁ : wellTypedPolicies ps₁ Γ = .some ps₁')
-  (hwt₂ : wellTypedPolicies ps₂ Γ = .some ps₂') :
+  (hwt₁ : wellTypedPolicies ps₁ Γ = .ok ps₁')
+  (hwt₂ : wellTypedPolicies ps₂ Γ = .ok ps₂') :
   ∃ asserts, verifyIsAuthorized φ ps₁' ps₂' (SymEnv.ofEnv Γ) = .ok asserts
 := by
   simp only [verifyIsAuthorized]
@@ -115,7 +110,7 @@ theorem verifyIsAuthorized_is_ok (φ : Term → Term → Term) {ps₁ ps₁' ps�
 /-- `verifyNeverErrors` succeeds on sufficiently well-formed inputs. -/
 theorem verifyNeverErrors_is_ok {p p' : Policy} {Γ : TypeEnv}
   (hwf : Γ.WellFormed)
-  (hwt : wellTypedPolicy p Γ = .some p') :
+  (hwt : wellTypedPolicy p Γ = .ok p') :
   ∃ asserts, verifyNeverErrors p' (SymEnv.ofEnv Γ) = .ok asserts
 := by
   exact verifyEvaluate_is_ok hwf hwt
@@ -123,69 +118,31 @@ theorem verifyNeverErrors_is_ok {p p' : Policy} {Γ : TypeEnv}
 /-- `verifyImplies` succeeds on sufficiently well-formed inputs. -/
 theorem verifyImplies_is_ok {ps₁ ps₁' ps₂ ps₂' : Policies} {Γ : TypeEnv}
   (hwf : Γ.WellFormed)
-  (hwt₁ : wellTypedPolicies ps₁ Γ = .some ps₁')
-  (hwt₂ : wellTypedPolicies ps₂ Γ = .some ps₂') :
+  (hwt₁ : wellTypedPolicies ps₁ Γ = .ok ps₁')
+  (hwt₂ : wellTypedPolicies ps₂ Γ = .ok ps₂') :
   ∃ asserts, verifyImplies ps₁' ps₂' (SymEnv.ofEnv Γ) = .ok asserts
 := by
   exact verifyIsAuthorized_is_ok _ hwf hwt₁ hwt₂
 
-private theorem compileWithEffect_allowAll_is_ok (effect : Effect) (Γ : TypeEnv) :
-  ∃ asserts, compileWithEffect effect verifyAlwaysAllows.allowAll (SymEnv.ofEnv Γ) = .ok asserts
+theorem isAuthorized_allowAll_is_ok (Γ : TypeEnv) :
+  isAuthorized [verifyAlwaysAllows.allowAll] (SymEnv.ofEnv Γ) = .ok (.prim (.bool .true))
 := by
-  simp only [compileWithEffect]
-  split
-  · simp [
-      verifyAlwaysAllows.allowAll,
-      Policy.toExpr,
-      Scope.toExpr,
-      PrincipalScope.toExpr,
-      ActionScope.toExpr,
-      ResourceScope.toExpr,
-      Conditions.toExpr,
-      compile,
-      compilePrim,
-      compileAnd,
-      Term.typeOf,
-      TermPrim.typeOf,
-      Factory.someOf,
-      Factory.ifSome,
-      Factory.ite,
-      Factory.noneOf,
-      Factory.ite.simplify,
-      Factory.isNone,
-      Factory.option.get,
-    ]
-  · simp
-
-private theorem satisfiedPolicies_allowAll_is_ok (effect : Effect) (Γ : TypeEnv) :
-  ∃ asserts, satisfiedPolicies effect [verifyAlwaysAllows.allowAll] (SymEnv.ofEnv Γ) = .ok asserts
-:= by
-  simp only [SymCC.satisfiedPolicies]
-  have ⟨_, h⟩ := compileWithEffect_allowAll_is_ok effect Γ
-  simp only [
-    h,
-    List.filterMapM, List.filterMapM.loop,
-    List.reverse_nil, List.reverse_cons,
-    List.nil_append, Except.bind_ok,
-  ]
-  split <;> simp
-
-private theorem isAuthorized_allowAll_is_ok (Γ : TypeEnv) :
-  ∃ asserts, isAuthorized [verifyAlwaysAllows.allowAll] (SymEnv.ofEnv Γ) = .ok asserts
-:= by
-  simp only [SymCC.isAuthorized]
-  have ⟨_, h₁⟩ := satisfiedPolicies_allowAll_is_ok .permit Γ
-  have ⟨_, h₂⟩ := satisfiedPolicies_allowAll_is_ok .forbid Γ
-  simp [h₁, h₂]
+  simp [SymCC.isAuthorized, SymCC.satisfiedPolicies, SymCC.compileWithEffect, verifyAlwaysAllows.allowAll]
+  simp [Policy.toExpr, PrincipalScope.toExpr, ActionScope.toExpr, ResourceScope.toExpr, Scope.toExpr, Conditions.toExpr]
+  simp [Factory.and, Factory.anyTrue, Factory.not, Factory.or]
+  simp [do_eq_ok, Factory.someOf]
+  exists (Term.prim (.bool true)).some
+  simp [Factory.eq, Factory.eq.simplify]
+  simp [SymCC.compile, compilePrim, Factory.someOf, compileAnd, Term.typeOf, TermPrim.typeOf, Factory.ifSome, Factory.ite, Factory.ite.simplify, Factory.noneOf, Factory.isNone, Factory.option.get, Factory.and, Factory.or, Factory.eq, Factory.eq.simplify, Factory.not]
 
 /-- `verifyAlwaysAllows` succeeds on sufficiently well-formed inputs. -/
 theorem verifyAlwaysAllows_is_ok {ps ps' : Policies} {Γ : TypeEnv}
   (hwf : Γ.WellFormed)
-  (hwt : wellTypedPolicies ps Γ = .some ps') :
+  (hwt : wellTypedPolicies ps Γ = .ok ps') :
   ∃ asserts, verifyAlwaysAllows ps' (SymEnv.ofEnv Γ) = .ok asserts
 := by
   have ⟨_, h₁⟩ := isAuthorized_is_ok hwf hwt
-  have ⟨_, h₂⟩ := isAuthorized_allowAll_is_ok Γ
+  have h₂ := isAuthorized_allowAll_is_ok Γ
   simp [
     verifyAlwaysAllows,
     verifyImplies,
@@ -196,7 +153,7 @@ theorem verifyAlwaysAllows_is_ok {ps ps' : Policies} {Γ : TypeEnv}
 /-- `verifyAlwaysDenies` succeeds on sufficiently well-formed inputs. -/
 theorem verifyAlwaysDenies_is_ok {ps ps' : Policies} {Γ : TypeEnv}
   (hwf : Γ.WellFormed)
-  (hwt : wellTypedPolicies ps Γ = .some ps') :
+  (hwt : wellTypedPolicies ps Γ = .ok ps') :
   ∃ asserts, verifyAlwaysDenies ps' (SymEnv.ofEnv Γ) = .ok asserts
 := by
   have ⟨_, h⟩ := isAuthorized_is_ok hwf hwt
@@ -210,8 +167,8 @@ theorem verifyAlwaysDenies_is_ok {ps ps' : Policies} {Γ : TypeEnv}
 /-- `verifyEquivalent` succeeds on sufficiently well-formed inputs. -/
 theorem verifyEquivalent_is_ok {ps₁ ps₁' ps₂ ps₂' : Policies} {Γ : TypeEnv}
   (hwf : Γ.WellFormed)
-  (hwt₁ : wellTypedPolicies ps₁ Γ = .some ps₁')
-  (hwt₂ : wellTypedPolicies ps₂ Γ = .some ps₂') :
+  (hwt₁ : wellTypedPolicies ps₁ Γ = .ok ps₁')
+  (hwt₂ : wellTypedPolicies ps₂ Γ = .ok ps₂') :
   ∃ asserts, verifyEquivalent ps₁' ps₂' (SymEnv.ofEnv Γ) = .ok asserts
 := by
   exact verifyIsAuthorized_is_ok _ hwf hwt₁ hwt₂
@@ -219,8 +176,8 @@ theorem verifyEquivalent_is_ok {ps₁ ps₁' ps₂ ps₂' : Policies} {Γ : Type
 /-- `verifyDisjoint` succeeds on sufficiently well-formed inputs. -/
 theorem verifyDisjoint_is_ok {ps₁ ps₁' ps₂ ps₂' : Policies} {Γ : TypeEnv}
   (hwf : Γ.WellFormed)
-  (hwt₁ : wellTypedPolicies ps₁ Γ = .some ps₁')
-  (hwt₂ : wellTypedPolicies ps₂ Γ = .some ps₂') :
+  (hwt₁ : wellTypedPolicies ps₁ Γ = .ok ps₁')
+  (hwt₂ : wellTypedPolicies ps₂ Γ = .ok ps₂') :
   ∃ asserts, verifyDisjoint ps₁' ps₂' (SymEnv.ofEnv Γ) = .ok asserts
 := by
   exact verifyIsAuthorized_is_ok _ hwf hwt₁ hwt₂
